Počiščen dokaz

06-formalizacija-dokazov/lambda.lean
@@ -18,48 +18,89 @@ inductive value : tm -> Prop
 | unit : value tm.unit
 | true : value tm.true
 | false : value tm.false
-| lam {x : nm} {N : tm} : value (tm.lam x N)
+| lam {x e} : value (tm.lam x e)
 
-def subst (x : nm) (M : tm) : tm -> tm
-| (tm.var y) := if x = y then M else tm.var y
-| tm.unit := tm.unit
-| tm.true := tm.true
-| tm.false := tm.false
-| (tm.app N1 N2) := tm.app (subst N1) (subst N2)
-| (tm.lam y N) := if x = y then tm.lam y N else tm.lam y (subst N)
-| (tm.if_then_else N N1 N2) := tm.if_then_else (subst N) (subst N1) (subst N2)
+def subst : nm -> tm -> tm -> tm
+| x e (tm.var y) :=
+    if x = y then e else tm.var y
+| x e tm.unit :=
+    tm.unit
+| x e tm.true :=
+    tm.true
+| x e tm.false :=
+    tm.false
+| x e (tm.app e1 e2) :=
+    tm.app (subst x e e1) (subst x e e2)
+| x e (tm.lam y e') :=
+    if x = y then tm.lam y e' else tm.lam y (subst x e e')
+| x e (tm.if_then_else e' e1 e2) :=
+    tm.if_then_else (subst x e e') (subst x e e1) (subst x e e2)
 
 inductive step : tm -> tm -> Prop
-| step1 {M M' N : tm} : step M M' -> step (tm.app M N) (tm.app M' N)
-| step2 {V N N' : tm} : value V -> step N N' -> step (tm.app V N) (tm.app V N')
-| beta {x} {M V : tm} : value V -> step (tm.app (tm.lam x M) V) (subst x V M)
-| test {M M' N1 N2 : tm} : step M M' -> step (tm.if_then_else M N1 N2) (tm.if_then_else M' N1 N2)
-| true {N1 N2 : tm} : step (tm.if_then_else tm.true N1 N2) N1
-| false {N1 N2 : tm} : step (tm.if_then_else tm.false N1 N2) N2
+| app1 {e1 e1' e2} :
+    step e1 e1' ->
+    step (tm.app e1 e2) (tm.app e1' e2)
+| app2 {v1 e2 e2'} :
+    value v1 ->
+    step e2 e2' ->
+    step (tm.app v1 e2) (tm.app v1 e2')
+| app_beta {x e1 v2} :
+    value v2 ->
+    step (tm.app (tm.lam x e1) v2) (subst x v2 e1)
+| if_then_else {e e' e1 e2} :
+    step e e' ->
+    step (tm.if_then_else e e1 e2) (tm.if_then_else e' e1 e2)
+| if_true {e1 e2} :
+    step (tm.if_then_else tm.true e1 e2) e1
+| if_false {e1 e2} :
+    step (tm.if_then_else tm.false e1 e2) e2
 
 inductive ctx : Type
 | nil : ctx
 | cons : nm -> ty -> ctx -> ctx
 
 inductive lookup : nm -> ctx -> ty -> Prop
-| here {x A Γ} : lookup x (ctx.cons x A Γ) A
-| there {x y : nm} {A B : ty} {Γ : ctx} : x ≠ y -> lookup x Γ A -> lookup x (ctx.cons y B Γ) A
+| here {x A Γ} :
+    lookup x (ctx.cons x A Γ) A
+| there {x y A B Γ} :
+    x ≠ y ->
+    lookup x Γ A ->
+    lookup x (ctx.cons y B Γ) A
 
 inductive of : ctx -> tm -> ty -> Prop
-| var {x Γ A}: lookup x Γ A -> of Γ (tm.var x) A
-| unit {Γ}: of Γ tm.unit ty.unit
-| true {Γ}: of Γ tm.true ty.bool
-| false {Γ}: of Γ tm.false ty.bool
-| app {Γ M N A B} : of Γ M (ty.arrow A B) -> of Γ N A -> of Γ (tm.app M N) B
-| lam {Γ x M A B} : of (ctx.cons x A Γ) M B -> of Γ (tm.lam x M) (ty.arrow A B)
-| if_then_else {Γ M N1 N2 A} : of Γ M ty.bool -> of Γ N1 A -> of Γ N2 A -> of Γ (tm.if_then_else M N1 N2) A
+| var {x Γ A} :
+    lookup x Γ A ->
+    of Γ (tm.var x) A
+| unit {Γ} :
+    of Γ tm.unit ty.unit
+| true {Γ} :
+    of Γ tm.true ty.bool
+| false {Γ} :
+    of Γ tm.false ty.bool
+| app {Γ e1 e2 A B} :
+    of Γ e1 (ty.arrow A B) ->
+    of Γ e2 A ->
+    of Γ (tm.app e1 e2) B
+| lam {Γ x e A B} :
+    of (ctx.cons x A Γ) e B ->
+    of Γ (tm.lam x e) (ty.arrow A B)
+| if_then_else {Γ e e1 e2 A} :
+    of Γ e ty.bool ->
+    of Γ e1 A ->
+    of Γ e2 A ->
+    of Γ (tm.if_then_else e e1 e2) A
 
-theorem substitution (Γ x A M M' A') : of Γ M A -> of (ctx.cons x A Γ) M' A' -> of Γ (subst x M M') A' :=
+theorem substitution {Γ x A e e' A'} :
+    of Γ e A
+    -> of (ctx.cons x A Γ) e' A'
+    -> of Γ (subst x e e') A'
+:=
 begin
   intros H,
   generalize ctx_cons : (ctx.cons x A Γ) = Γ',
   intros H',
   induction H',
+  repeat {simp},
   case of.var {
       rewrite <- ctx_cons at H'_a,
       unfold subst,
@@ -75,127 +116,154 @@ begin
       }
   },
   case of.unit {
-      unfold subst,
       apply of.unit
   },
   case of.true {
-      unfold subst,
       apply of.true
   },
   case of.false {
-      unfold subst,
       apply of.false
   },
   case of.app {
-      unfold subst,
       apply of.app,
       apply H'_ih_a ctx_cons,
-      apply H'_ih_a_1 ctx_cons,
+      apply H'_ih_a_1 ctx_cons
   },
   case of.if_then_else {
-      unfold subst,
       apply of.if_then_else,
       apply H'_ih_a ctx_cons,
       apply H'_ih_a_1 ctx_cons,
-      apply H'_ih_a_2 ctx_cons,
+      apply H'_ih_a_2 ctx_cons
   },
   case of.lam {
       unfold subst,
       by_cases (x = H'_x),
         simp [h], apply of.lam, sorry,
-        simp [h], apply of.lam, sorry,
+        simp [h], apply of.lam, sorry
   },
 end
 
-theorem preservation (Γ M M') : step M M' -> forall A, of Γ M A -> of Γ M' A :=
+theorem preservation {e e'} :
+    step e e' ->
+    forall {Γ A}, of Γ e A ->
+    of Γ e' A
+:=
 begin
     intros Hstep,
     induction Hstep,
-    repeat {intros A Hof},
-    case step.beta
-        {cases Hof, cases Hof_a, apply substitution _ _ _ _ _ _ Hof_a_1 Hof_a_a },
-    case step.step1
-        {cases Hof, apply of.app,
-            apply Hstep_ih _ Hof_a, apply Hof_a_1},
-    case step.step2
-        {cases Hof, apply of.app, apply Hof_a, apply Hstep_ih _ Hof_a_1},
-    case step.test {
+    repeat {intros Γ A Hof},
+    case step.app_beta {
+        cases Hof,
+        cases Hof_a,
+        apply substitution Hof_a_1 Hof_a_a
+    },
+    case step.app1 {
+        cases Hof,
+        apply of.app,
+        apply Hstep_ih Hof_a,
+        apply Hof_a_1
+    },
+    case step.app2 {
+        cases Hof,
+        apply of.app,
+        apply Hof_a,
+        apply Hstep_ih Hof_a_1
+    },
+    case step.if_then_else {
         cases Hof,
         apply of.if_then_else,
-        apply Hstep_ih _ Hof_a,
+        apply Hstep_ih Hof_a,
         apply Hof_a_1,
         apply Hof_a_2
     },
-    case step.true {
+    case step.if_true {
         cases Hof,
         apply Hof_a_1
     },
-    case step.false {
+    case step.if_false {
         cases Hof,
         apply Hof_a_2
     }
 end
 
-theorem progress (M A) : of ctx.nil M A -> (value M) ∨ (exists M', step M M') :=
+theorem progress {e A} :
+    of ctx.nil e A ->
+    (value e) ∨ (exists e', step e e')
+:=
 begin
     generalize empty : ctx.nil = Γ,
     intros H,
     induction H,
-    case of.var
-        {rewrite ←empty at H_a, cases H_a},
-    case of.unit
-        {left, exact value.unit},
-    case of.app
-        {
-            cases H_ih_a empty,
-                case or.inl {
-                    cases H_a,
-                        case of.var
-                            {rw ←empty at H_a_a, cases H_a_a},
-                        case of.app
-                            {cases h},
-                        case of.lam {
-                            cases H_ih_a_1 empty,
-                            right,
-                            existsi (subst H_a_x H_N H_a_M),
-                            apply step.beta,
-                            assumption,
-                            right,
-                            cases h_1,
-                            existsi (tm.app (tm.lam H_a_x H_a_M) h_1_w),
-                            eapply step.step2,
-                            exact value.lam,
-                            assumption
-                        },
-                        case of.if_then_else {
-                            cases h
-                        }
-                },
-                case or.inr {
-                    cases h with M H_step,
-                    right,
-                    existsi (tm.app M H_N),
-                    apply step.step1,
-                    assumption
-                }
-        },
-    case of.lam
-        {left, exact value.lam},
-    case of.true
-        {left, exact value.true},
-    case of.false
-        {left, exact value.false},
-    case of.if_then_else {
+    case of.var {
+        rewrite ←empty at H_a,
+        cases H_a
+    },
+    case of.unit {
+        left,
+        exact value.unit
+    },
+    case of.app {
         cases H_ih_a empty,
         case or.inl {
             cases H_a,
             case of.var
                 {rw ←empty at H_a_a, cases H_a_a},
+            case of.app
+                {cases h},
+            case of.lam {
+                cases H_ih_a_1 empty,
+                right,
+                existsi (subst H_a_x H_e2 H_a_e),
+                apply step.app_beta,
+                assumption,
+                right,
+                cases h_1,
+                existsi (tm.app (tm.lam H_a_x H_a_e) h_1_w),
+                eapply step.app2,
+                exact value.lam,
+                assumption
+            },
+            case of.if_then_else {
+                cases h
+            }
+        },
+        case or.inr {
+            cases h with e H_step,
+            right,
+            existsi (tm.app e H_e2),
+            apply step.app1,
+            assumption
+        }
+    },
+    case of.lam {
+        left,
+        exact value.lam
+    },
+    case of.true {
+        left,
+        exact value.true
+    },
+    case of.false {
+        left,
+        exact value.false
+    },
+    case of.if_then_else {
+        cases H_ih_a empty,
+        case or.inl {
+            cases H_a,
+            case of.var {
+                rw ←empty at H_a_a,
+                cases H_a_a
+            },
             case of.true {
-                right, existsi H_N1, exact step.true
+                right,
+                existsi H_e1,
+                exact step.if_true
             },
             case of.false {
-                right, existsi H_N2, exact step.false
+                right,
+                existsi H_e2,
+                exact step.if_false
             },
             cases h,
             cases h
@@ -203,9 +271,8 @@ begin
         case or.inr {
             cases h,
             right,
-            existsi (tm.if_then_else h_w H_N1 H_N2),
-            exact (step.test h_h),
+            existsi (tm.if_then_else h_w H_e1 H_e2),
+            exact (step.if_then_else h_h),
         }
     }
 end
-
